transformation/proofs/GenerateArchitectureFacts.v
@@ -1,6 +1,5 @@
 (** * Facts about Architecture Generation *)
 
-Require Import String.
 Require Import common.CoqLib.
 Require Import common.GlobalFacts.
 Require Import common.StateAndErrorMonad.
@@ -13,11 +12,10 @@ Require Import common.proofs.ListPlusFacts.
 Require Import sitpn.SitpnLib.
 Require Import sitpn.SitpnFacts.
 
-Require Import hvhdl.Place.
 Require Import hvhdl.AbstractSyntax.
+Require Import hvhdl.WellDefinedDesign.
 
 Require Import transformation.Sitpn2HVhdl.
-Require Import transformation.proofs.GenerateArchitectureInvs.
 Require Import transformation.proofs.SInvTactics.
 
 (** ** Facts about the generation of PCIs *)
@@ -40,7 +38,7 @@ Section GenPCIsFacts.
   
   (** *** Facts about the [generate_pci] function *)
 
-  Lemma p_comp_ex_Peq_equiv :
+  Lemma pci_ex_Peq_equiv :
     forall sitpn (x y : P sitpn) s,
       Peq x y ->
       ((exists id__p g__p i__p o__p,
@@ -53,7 +51,7 @@ Section GenPCIsFacts.
        exists id__p, g__p, i__p, o__p; split; [ eauto with setoidl | assumption ]).
   Qed.
   
-  Lemma gen_pci_p_comp_ex :
+  Lemma gen_pci_pci_ex :
     forall sitpn (n : nat) (a : P sitpn) (s1 : Sitpn2HVhdlState sitpn) (x : unit) (s2 : Sitpn2HVhdlState sitpn),
       generate_pci a n s1 = OK x s2 ->
       exists id__p g__p i__p o__p,
@@ -63,7 +61,7 @@ Section GenPCIsFacts.
     all: do 4 eexists; split; [ eauto with setoidl | left; eauto ].
   Qed.  
 
-  Lemma gen_pci_p_comp_ex_inv :
+  Lemma gen_pci_pci_ex_inv :
     forall sitpn (n : nat) (a : P sitpn) (s1 : Sitpn2HVhdlState sitpn) (x : unit) (s2 : Sitpn2HVhdlState sitpn),
       generate_pci a n s1 = OK x s2 ->
       forall b,
@@ -75,9 +73,9 @@ Section GenPCIsFacts.
     intros *; intros e b; destruct (Peqdec a b) as [Peq_ab | nPeq_ab]. 
 
     (* CASE [Peq a b], implies [Q a s' <-> Q b s']. *)
-    - rewrite <- (p_comp_ex_Peq_equiv sitpn a b s1 Peq_ab).
-      rewrite <- (p_comp_ex_Peq_equiv sitpn a b s2 Peq_ab).
-      intro; eapply gen_pci_p_comp_ex; eauto.
+    - rewrite <- (pci_ex_Peq_equiv sitpn a b s1 Peq_ab).
+      rewrite <- (pci_ex_Peq_equiv sitpn a b s2 Peq_ab).
+      intro; eapply gen_pci_pci_ex; eauto.
       
     (* CASE [~Peq a b], then nevermind the new entry [(a, id__p)] and new
      PCI in [(beh s2)]. *)
@@ -94,7 +92,7 @@ Section GenPCIsFacts.
 
   (** *** Facts about the [generate_pcis] function *)
   
-  Lemma gen_pcis_p_comp_ex :
+  Lemma gen_pcis_pci_ex :
     forall (sitpn : Sitpn) (b : P sitpn -> nat) (s : Sitpn2HVhdlState sitpn) v s' p,
       generate_pcis b s = OK v s' ->
       Sig_in_List (lofPs s) ->
@@ -107,14 +105,14 @@ Section GenPCIsFacts.
     eapply iter_prop_A_state with (eqA := Peq); eauto.
 
     (* Proves that [Peq a b] implies [Q a s' <-> Q b s']. *)
-    - eapply p_comp_ex_Peq_equiv.
+    - eapply pci_ex_Peq_equiv.
       
     (* Proves that [∀ a, f a s = OK v s' -> Q a s'] where [f] 
      is [generate_pci] here. *)
-    - cbn; intros x; eapply gen_pci_p_comp_ex.
+    - cbn; intros x; eapply gen_pci_pci_ex.
       
     (* Proves that property [Q] is invariant. *)
-    - simpl; intros x; eapply gen_pci_p_comp_ex_inv with (n := b x).
+    - simpl; intros x; eapply gen_pci_pci_ex_inv with (n := b x).
 
     (* Proves that *)
     - eapply SIL_forall_A; eauto.
@@ -127,6 +125,25 @@ End GenPCIsFacts.
 Section GenTCIsFacts.
 
   (** *** Facts about the [generate_tcis] function *)
+
+  Lemma gen_tcis_pci_ex :
+    forall (sitpn : Sitpn) (s : Sitpn2HVhdlState sitpn) v s' p,
+      generate_tcis s = OK v s' ->
+      (exists id__p g__p i__p o__p,
+          InA Pkeq (p, id__p) (p2pcomp (γ s))
+          /\ InCs (cs_comp id__p Petri.place_entid g__p i__p o__p) (beh s)) -> 
+      (exists id__p g__p i__p o__p,
+          InA Pkeq (p, id__p) (p2pcomp (γ s'))
+          /\ InCs (cs_comp id__p Petri.place_entid g__p i__p o__p) (beh s')).
+  Proof. intros *; intros H; pattern s, s'; solve_sinv_pattern.
+         match goal with
+         | [ EQ: OK _ _ = OK _ _ |- _ ] =>
+             inversion EQ; subst; cbn
+         end;
+         destruct 1 as [id__p [g__p [i__p [o__p [InA_ InCs_] ] ] ] ].
+         exists id__p, g__p, i__p, o__p; split; [ assumption | (right; assumption) ].
+  Qed.
+
   
 End GenTCIsFacts.
 
@@ -134,7 +151,25 @@ End GenTCIsFacts.
 
 Section GenArchiFacts.
 
-  Lemma gen_archi_p_comp_ex :
+  Lemma gen_arch_inv_lofPs :
+    forall {sitpn mm s v s'},
+      @generate_architecture sitpn mm s = OK v s' ->
+      lofPs s = lofPs s'.
+  Proof. intros *; intros H; pattern s, s'; solve_sinv_pattern. Qed.
+
+  Lemma gen_arch_inv_lofTs :
+    forall {sitpn mm s v s'},
+      @generate_architecture sitpn mm s = OK v s' ->
+      lofTs s = lofTs s'.
+  Proof. intros *; intros H; pattern s, s'; solve_sinv_pattern. Qed.
+
+  Lemma gen_arch_inv_sil_lofTs :
+    forall {sitpn mm s v s'},
+      @generate_architecture sitpn mm s = OK v s' ->
+      Sig_in_List (lofTs s) -> Sig_in_List (lofTs s').
+  Proof. intros *; intros H; pattern s, s'; solve_sinv_pattern. Qed.
+  
+  Lemma gen_archi_pci_ex :
     forall (sitpn : Sitpn) (b : P sitpn -> nat) (s : Sitpn2HVhdlState sitpn) v s' p,
       generate_architecture b s = OK v s' ->
       Sig_in_List (lofPs s) ->
@@ -143,9 +178,18 @@ Section GenArchiFacts.
           /\ InCs (cs_comp id__p Petri.place_entid g__p i__p o__p) (beh s')).
   Proof.
     intros *; intros e; monadInv e; intros SIL_lofPs.
-    eapply gen_tcis_p_comp_ex; eauto.
-    eapply gen_pcis_p_comp_ex; eauto.
+    eapply gen_tcis_pci_ex; eauto.
+    eapply gen_pcis_pci_ex; eauto.
   Qed.
+
+  Lemma gen_archi_nodup_cids :
+    forall (sitpn : Sitpn) (b : P sitpn -> nat)
+           (s : Sitpn2HVhdlState sitpn) v s',
+      generate_architecture b s = OK v s' ->
+      (forall id__c, In id__c (get_cids (beh s)) -> id__c < nextid s) ->
+      NoDup (get_cids (beh s)) ->
+      NoDup (get_cids (beh s')).
+  Admitted.
   
 End GenArchiFacts.
 
