transformation/proofs/Sitpn2HVhdlInvs.v
@@ -1,4 +1,3 @@
 Require Export transformation.proofs.GenerateInfosInvs.
-Require Export transformation.proofs.GenerateArchitectureInvs.
 Require Export transformation.proofs.GeneratePortsInvs.
 Require Export transformation.proofs.GenerateHVhdlInvs.
